

Week 4. By Deng Yufan.

Prob 1. Prove the following are not RL.

a. $A = \{0^n 1^m \mid n \leq m\}$.

If A is a RL, then:

Using pumping lemma, there is a n satisfying the condition in lemma.

So $0^n 1^n \in A$. $\exists x = 0^p, y = 0^q, z = 0^{n-p-q} 1^n$ ($p+q \leq n$), $xy^*z \in A$.

But $xy^2z = 0^{n+q} 1^n \notin A$.

b. $B = \{0^n 1 0^n \mid n \geq 1\}$.

If B is a RL, then use the pumping lemma.

$|0^n 1 0^n| \geq n$, $0^n 1 0^n \in B$. then $\exists x = 0^p, y = 0^q, z = 0^{n-p-q} 1 0^n$. $xy^*z \in B$.

But $xz = 0^{n-q} 1 0^n \notin B$.

c. $C = \{w^2 \mid w \in \{0,1\}^*\}$.

If C is a RL, then use the pumping lemma.

$|0^n 1 0^n| \geq n$, $0^n 1 0^n \in C$. then $\exists x = 0^p, y = 0^q, z = 0^{n-p-q} 1 0^n$. $xy^*z \in C$.

But $xz = 0^{n-q} 1 0^n \notin C$, ^{otherwise} ~~since~~ the end of w is 1, but $0^{n-q} 1 \neq 0^n 1$.

d. $D = \{ww^R \mid w \in \{0,1\}^*\}$.

If D is a RL, then use the pumping lemma.

$|0^n 1 1 0^n| \geq n$, $0^n 1 1 0^n \in D$. then $\exists x = 0^p, y = 0^q, z = 0^{n-p-q} 1 1 0^n$. $xy^*z \in D$.

But $xz = 0^{n-q} 1 1 0^n \notin D$, since the only two 1 are not symmetrical.



Prob 2. a. If L is a language, and a is a symbol, ~~then~~ $L \setminus a = \{w \mid wa \in L\}$.

Prove L is ~~RL~~ $\Rightarrow L \setminus a$ is RL.

We prove L can be presented as RE $\Rightarrow L \setminus a$ can be represented as RE by induction the structure of RE.

As base, we have $\emptyset \setminus a = \emptyset$ is RE. $\epsilon \setminus a = \emptyset$ is RE. $b \setminus a = \emptyset$ ($b \neq a$) is RE.

$a \setminus a = \{\epsilon\}$ is RE.

As induction, if E, F is RE, $L(E) \setminus a, L(F) \setminus a$ can be represented as RE E' and F' , respectively. then:

$$\begin{aligned} L(E+F) \setminus a &= \{w \mid wa \in L(E) \text{ or } wa \in L(F)\} \\ &= \{w \mid wa \in L(E)\} \cup \{w \mid wa \in L(F)\} \\ &= L(E'+F') \end{aligned}$$

$$\begin{aligned} L(EF) \setminus a &= \{w \mid wa \in L(EF)\} \\ &= \{xy \mid \begin{matrix} x \in L(E), y \in L(F) \\ \text{at the end of } x \end{matrix}\} \cup \{w \mid wa \in L(E), \epsilon \in L(F)\}. \end{aligned}$$

so if $\epsilon \in L(F)$, $L(EF) \setminus a = L(EF'+E')$, else $L(EF) \setminus a = L(EF')$.

$$\begin{aligned} L(E^*) \setminus a &= \{w \mid wa \in \bigcup_{i=0}^{+\infty} L(E)^i\} \\ &= \bigcup_{i=0}^{+\infty} \{w \mid wa \in L(E)^i\} \end{aligned}$$

if $\exists w_0, wa_0 \in L(E)$, discussing a is ~~at the end of~~ which $L(E)$, we have

$$\begin{aligned} \text{LHS} &= \bigcup_{i=0}^{+\infty} \{w \mid w \in L(E)^i, [L(E) \setminus a]\} \\ &= L(E^*E'). \end{aligned}$$

else $\forall w, wa \notin L(E)$, then $wa \notin L(E)^*$.

$$L(E^*) \setminus a = L(\emptyset).$$

So $E+F, EF, E^*$ is closed under $L(E) \setminus a$.



b. Let $a_1L = \{w \mid aw \in L\}$. Prove L is RL $\Rightarrow a_1L$ is RL.

We provide a better method than (a).

Let DFA $M = (Q, \Sigma, \delta, q_0, F)$. $L(M) = A$. We can assume $a \in \Sigma$, otherwise $a_1L = \emptyset$ is RL.

Let DFA $M' = (Q, \Sigma, \delta', q_1, F)$ which $\delta'(q, a) = \delta(q, a)$ and $q_1 = \delta(q_0, a)$.

We prove $aw \in L(M) \Leftrightarrow w \in L(M')$.

$$\Rightarrow: aw \in L(M) \Rightarrow \hat{\delta}(q_0, aw) \in F \Rightarrow \hat{\delta}(\hat{\delta}(q_0, a), w) \in F \\ \Rightarrow \hat{\delta}'(q_1, w) \in F \Rightarrow w \in L(M').$$

$$\Leftarrow: w \in L(M') \Rightarrow \hat{\delta}'(q_1, w) \in F \Rightarrow \hat{\delta}(q_0, aw) \in F \Rightarrow aw \in L(M).$$

So a_1L is RL.

Prob 3. Prove the RL is closed under following operations.

a. $\text{min}(L) = \{w \mid w \in L, \text{ but no proper prefix of } w \text{ is in } L\}$.

Let DFA $M = (Q, \Sigma, \delta, q_0, F)$, $L(M) = L$.

Let NFA $M' = (Q, \Sigma, \delta', q_0, F)$. $\delta'(q, a) = \begin{cases} \delta(q, a) & (q \notin F) \\ \emptyset & (q \in F) \end{cases}$.

We prove $L(M') = \text{min}(L)$, or say $w \in L$, but no proper prefix of w is in $L \Leftrightarrow w \in L(M')$.

First $\hat{\delta}'(q_0, \epsilon) = \{q_0\}$. $\Rightarrow: w \in L \Rightarrow \hat{\delta}(q_0, w) \in F$.

$\hat{\delta}'(q_0, w) = \{\hat{\delta}(q_0, w)\}$. no proper prefix of w is in $L \Rightarrow \hat{\delta}(q_0, xy) \notin F$, if $xy = w, y \neq \emptyset$.

$\hat{\delta}'(q_0, w) = \{\hat{\delta}(q_0, w)\}$. By induction, we can easily prove $\hat{\delta}'(q_0, w) = \{\hat{\delta}(q_0, w)\}$.

Since w is proper prefix of w , $\hat{\delta}(q_0, w) \notin F$. so $\hat{\delta}'(q_0, w) \cap F \neq \emptyset$. $w \in L(M')$.

So $\hat{\delta}'(q_0, w) = \{\hat{\delta}(q_0, w)\}$. $\Leftarrow: \text{If } xy = w, y \neq \emptyset, x \in L$, then $\hat{\delta}(q_0, x) \in F$.



We first prove $\hat{f}'(q_0, w) \subseteq [\hat{f}(q_0, w)]$.

Induction the length of w . we have $\hat{f}'(q_0, \epsilon) = \{q_0\} = [\hat{f}(q_0, \epsilon)]$.

if $\hat{f}'(q_0, w) \subseteq [\hat{f}(q_0, w)]$, then $\hat{f}'(q_0, wa) = \bigcup_{q \in \hat{f}'(q_0, w)} \hat{f}'(q, a)$.

if $\hat{f}'(q_0, w) = \emptyset$, then $\hat{f}'(q_0, wa) = \emptyset$. (1)

if $\hat{f}'(q_0, w) = [\hat{f}(q_0, w)]$, then $\hat{f}'(q_0, wa) = \hat{f}'(\hat{f}(q_0, w), a)$.

if $\hat{f}(q_0, w) \in F$, then $\hat{f}'(q_0, wa) = \emptyset$. (2)

if $\hat{f}(q_0, w) \notin F$, then $\hat{f}'(q_0, wa) = [\hat{f}(\hat{f}(q_0, w), a)] = [\hat{f}(q_0, wa)]$. (3)

So $\hat{f}'(q_0, wa) \subseteq [\hat{f}(q_0, wa)]$.

We prove $w \in L$, but no proper prefix of w is in $L \Leftrightarrow w \in L(M')$ - this ends the proof.

\Rightarrow : $w \in L \Rightarrow \hat{f}(q_0, w) \in F$.

no proper prefix of w is in $L \Rightarrow$ write w as xy ^($y \neq \epsilon$) $x \notin L$.

$\Rightarrow \hat{f}(q_0, x) \notin F$.

According to the proof above, ^{when it is only possible to be (3).} we have $\hat{f}'(q_0, w) = [\hat{f}(q_0, w)]$, ~~(1)~~ then $\hat{f}'(q_0, w) \cap F \neq \emptyset$.

\Leftarrow : $w \in L(M') \Rightarrow \hat{f}'(q_0, w) \cap F \neq \emptyset \Rightarrow \hat{f}'(q_0, w) = [\hat{f}(q_0, w)]$.

$\Rightarrow \hat{f}(q_0, w) \in F \Rightarrow$ ~~$w \in L$~~ ^{an} $w \in L$.

if $xy = w$, $y \neq \epsilon$, $x \in L$, then $\hat{f}(q_0, x) \in F$.

if $\hat{f}'(q_0, x) = \emptyset$, $\hat{f}'(q_0, xa) = \emptyset$.

if $\hat{f}'(q_0, x) = [\hat{f}(q_0, x)]$, $\hat{f}'(q_0, xa) = \emptyset$.

So $\hat{f}'(q_0, xa) = \emptyset$, thus $\hat{f}'(q_0, xy) = \emptyset$. So $w \notin L(M')$, contradiction.

So no proper prefix of w is in L .



b. $\max(L) = \{w \mid \text{no nonempty string } x \text{ that } wx \in L\}$.

~~We prove $\max(L) = \complement \min(L)$, where \complement is complement operation.~~

~~$\min(L) = \{w \mid w \in L, \text{ but there is no all proper prefix of } w \text{ is in } L\}$.~~

Consider DFA $M = (Q, \Sigma, \delta, q_0, F)$.

~~If for all $w \in L$, $\delta(q_0, w) \in F$~~ Let DFA $M' = (Q, \Sigma, \delta, q_0, F')$.

$$F' = \{q \in F \mid \forall q' \in F, w \neq \epsilon, \delta(q, w) \neq q'\}.$$

We proof $w \in L$, no nonempty string x that $wx \in L \Leftrightarrow w \in L(M')$.

\Rightarrow : $w \in L \Rightarrow \delta(q_0, w) \in F$. If $\delta(q_0, w) \notin F'$, then $\exists q' \in F, w' \neq \epsilon, \delta(\delta(q_0, w), w') = q'$.

then $\delta(q_0, ww') = q' \in F$, so $ww' \in L$, contradiction. So $\delta(q_0, w) \in F'$.
 $w \in L(M')$

\Leftarrow : $w \in L(M') \Rightarrow \delta(q_0, w) \in F' \subseteq F \Rightarrow w \in L$.

For any $x \neq \epsilon, q' \in F, \delta(q_0, wx) = \delta(\delta(q_0, w), x) \neq q'$.

So no nonempty string x that $wx \in L$.

c. $\text{init}(L) = \{w \mid \exists x, wx \in L\}$.

Induction the structure of RE.

As basis. $\text{init}(L(\emptyset)) = L(\emptyset)$, $\text{init}(L(\epsilon)) = L(\epsilon)$, $\text{init}(L(a)) = L(\epsilon + a)$.

If E, F is RE. $\text{init}(L(E)) = L(E')$, $\text{init}(L(F)) = L(F')$.

~~$\text{init}(L(E)) = L(E')$~~ $\text{init}(L(E+F)) = L(E' + F')$.

$\text{init}(L(EF)) = L(EF' + E')$. since we can discuss if x takes up all $L(F)$.

$\text{init}(L(E^*)) = L(E^*E' + \epsilon)$.

$$\begin{aligned} \text{since } \text{init}(L(E^*)) &= \bigcup_{n=0}^{+\infty} \text{init}(L(E^n)) = \bigcup_{n=0}^{+\infty} \text{init}(L(E^{n-1}E)) \cup L(E) \\ &= \bigcup_{n=1}^{+\infty} L(E^{n-1}E' + (E^{n-1})') \cup L(E) \\ &= \bigcup_{n=1}^{+\infty} L(E^{n-1}E') \cup L(E) \\ &= L(E^*E' + \epsilon). \end{aligned}$$



Prob 4. Let $\text{half}(L) = \{w \mid \exists x, |x|=|w|, wx \in L\}$. Prove L is RL $\Rightarrow \text{half}(L)$ is RL.

Let DFA $M = (Q, \Sigma, \delta, q_0, F)$. $L(M) = L$.

Let DFA $M' = (Q \times 2^Q, \Sigma, \delta', (q_0, F), F' = \{(q, s) \mid s \in Q, q \in F\})$.

where $\delta'(q, s, a) = (\delta(q, a), \bigcup_{|c|=1} \bigcup_{\delta(q', c) \in S} \{q'\})$.

We first prove $\hat{\delta}'(q, s, w) = (\hat{\delta}(q, w), \bigcup_{|c|=|w|} \bigcup_{\delta(q', c) \in S} \{q'\})$.

Induction the length of w . we have $\hat{\delta}'(q, s, \epsilon) = (q, s) = (\hat{\delta}(q, \epsilon), \bigcup_{|c|=0} \bigcup_{\delta(q', c) \in S} \{q'\})$.

If $\hat{\delta}'(q, s, w) = (\hat{\delta}(q, w), \bigcup_{|c|=|w|} \bigcup_{\delta(q', c) \in S} \{q'\})$. we prove $\hat{\delta}'(q, s, wa) = (\hat{\delta}(q, wa), \bigcup_{|c|=|w|+1} \bigcup_{\delta(q', c) \in S} \{q'\})$.

We have $\hat{\delta}'(q, s, wa) = \delta'(\hat{\delta}'(q, s, w), a)$

$\Leftarrow: w \in L(M') \Rightarrow \hat{\delta}'(q_0, F, w) \in F'$.

$\Rightarrow \hat{\delta}(q, w) \in \bigcup_{|c|=|w|} \bigcup_{\delta(q', c) \in F} \{q'\}$.

So $\exists |c|=|w|, \hat{\delta}(\hat{\delta}(q, w), c) \in F$.

that is $\hat{\delta}(q, wc) \in F, wc \in L$.

Consider $x=c$, we have $|x|=|w|, wx \in L$.

$= \delta'(\hat{\delta}(q, w), \bigcup_{|c|=|w|} \bigcup_{\delta(q', c) \in S} \{q'\}, a)$

$= (\hat{\delta}(\hat{\delta}(q, w), a), \bigcup_{|c'|=1} \bigcup_{\delta(q', c) \in S} \bigcup_{|c|=|w|} \bigcup_{\delta(q'', c') \in S} \{q''\})$.

$= (\hat{\delta}(q, wa), \bigcup_{|c|=1} \bigcup_{|c'|=|w|} \bigcup_{\delta(\hat{\delta}(q', a), c') \in S} \{q'\})$

$= (\hat{\delta}(q, wa), \bigcup_{|c|=1} \bigcup_{|c'|=|w|} \bigcup_{\delta(q', cc') \in S} \{q'\})$.

$= (\hat{\delta}(q, wa), \bigcup_{|c|=|w|+1} \bigcup_{\delta(q', c) \in S} \{q'\})$.

Now we prove $L(M') = \text{half}(L)$. which is $\exists x, |x|=|w|, wx \in L \Leftrightarrow w \in L(M')$.

$\Rightarrow: wx \in L \Rightarrow \hat{\delta}(q_0, wx) \in F$. Let $q = \hat{\delta}(q_0, w)$, then $\hat{\delta}(q, x) \in F$.

Let $S = \bigcup_{|q|=|w|} \bigcup_{\delta(q', c) \in F} \{q'\}$.
then $\hat{\delta}'(q_0, F, w) = (\hat{\delta}(q_0, w), \bigcup_{|c|=|w|} \bigcup_{\delta(q', c) \in F} \{q'\}) = (q, S)$.

Since $|wx|=|w|, \hat{\delta}(q, x) \in F$. So consider $c=x, q'=q$. we have $q \in S$. then $(q, S) \in F'$.

So $\hat{\delta}'(q_0, F, w) \in F'$. $w \in L(M')$.

